CrVal.v
@@ -1,0 +1,131 @@
+From MyProject Require Import MyInts.
+From MyProject Require Import Integers.
+
+Inductive CrVal : Type :=
+| CrInt (val : uint8)
+| CrPtr (base : uintptr) (offset : uintptr)
+| CrNil.
+
+Definition eqb (x y : CrVal) : bool :=
+  match x, y with
+  | CrInt x', CrInt y' => Integers.eq x' y'
+  | CrPtr b1 o1, CrPtr b2 o2 =>
+    (Integers.eq b1 b2) &&
+    (Integers.eq o1 o2)
+  | CrNil, CrNil => true
+  | _, _ => false
+  end.
+
+Definition add (x y : CrVal) : CrVal :=
+  match x, y with
+  | CrInt x', CrInt y' =>
+    (CrInt (Integers.add x' y'))
+  | CrPtr b' o', CrInt y_ =>
+    let y' : uintptr := repr (intval y_) in
+    (CrPtr b' (Integers.add o' y'))
+  | _, _ => CrNil
+  end.
+
+Definition sub (x y : CrVal) : CrVal :=
+  match x, y with
+  | CrInt x', CrInt y' =>
+    (CrInt (Integers.sub x' y'))
+  | CrPtr b' o', CrInt y_ =>
+    let y' : uintptr := repr (intval y_) in
+    (CrPtr b' (Integers.sub o' y'))
+  | _, _ => CrNil
+  end.
+
+Definition and (x y : CrVal) : CrVal :=
+  match x, y with
+  | CrInt x', CrInt y' =>
+    (CrInt (Integers.and x' y'))
+  | _, _ => CrNil
+  end.
+
+Definition or (x y : CrVal) : CrVal :=
+  match x, y with
+  | CrInt x', CrInt y' =>
+    (CrInt (Integers.or x' y'))
+  | _, _ => CrNil
+  end.
+
+Definition xor (x y : CrVal) : CrVal :=
+  match x, y with
+  | CrInt x', CrInt y' =>
+    (CrInt (Integers.xor x' y'))
+  | _, _ => CrNil
+  end.
+
+Definition not (x : CrVal) : CrVal :=
+  match x with
+  | CrInt x' =>
+    (CrInt (Integers.not x'))
+  | _ => CrNil
+  end.
+
+Definition mul (x y : CrVal) : CrVal :=
+  match x, y with
+  | CrInt x', CrInt y' =>
+    (CrInt (Integers.mul x' y'))
+  | _, _ => CrNil
+  end.
+
+Definition divu (x y : CrVal) : CrVal :=
+  match x, y with
+  | CrInt x', CrInt y' =>
+    (CrInt (Integers.divu x' y'))
+  | _, _ => CrNil
+  end.
+
+Definition modu (x y : CrVal) : CrVal :=
+  match x, y with
+  | CrInt x', CrInt y' =>
+    (CrInt (Integers.modu x' y'))
+  | _, _ => CrNil
+  end.
+
+Lemma crval_concrete_if_else : forall (v1 v2 : CrVal),
+  ((if eqb v1 v2 then true else false) = true)->
+  v1 = v2.
+Proof.
+  intros v1 v2 H.
+  destruct v1, v2; try discriminate.
+  - unfold eqb in H.
+    unfold eq in H.
+    unfold Rocqlib.zeq in H.
+    destruct (BinInt.Z.eq_dec (unsigned val) (unsigned val0)).
+    + apply uintw_eq_from_unsigned in e.
+      rewrite e.
+      reflexivity.
+    + exfalso. congruence.
+  - unfold eqb in H.
+    unfold eq in H.
+    unfold Rocqlib.zeq in H.
+    destruct (BinInt.Z.eq_dec (unsigned base) (unsigned base0));
+    destruct (BinInt.Z.eq_dec (unsigned offset) (unsigned offset0));
+    simpl in *.
+    + apply uintw_eq_from_unsigned in e.
+      apply uintw_eq_from_unsigned in e0.
+      rewrite e. rewrite e0. reflexivity.
+    + exfalso. congruence.
+    + exfalso. congruence.
+    + exfalso. congruence.
+  - reflexivity.
+Qed.
+
+Lemma crval_concrete_if_else2 : forall (v1 v2 : CrVal),
+  ((if eqb v1 v2 then true else false) = false)->
+  v1 <> v2.
+Proof with congruence.
+  intros v1 v2 H.
+  destruct v1, v2; try discriminate;
+  unfold eqb in H;
+  unfold eq in H;
+  unfold Rocqlib.zeq in H.
+  - destruct (BinInt.Z.eq_dec (unsigned val) (unsigned val0));
+    try injection...
+  - destruct (BinInt.Z.eq_dec (unsigned base) (unsigned base0));
+    destruct (BinInt.Z.eq_dec (unsigned offset) (unsigned offset0));
+    simpl in *; try injection...        
+Qed.
