MyInts.v
@@ -5,12 +5,12 @@ Require Import ZArith.
 Definition uint8   := @bit_int  8%positive.
 Definition uintptr := @bit_int 32%positive.
 
-Lemma uint8_eq_from_unsigned : forall (v1 v2 : uint8),
+Lemma uintw_eq_from_unsigned :
+  forall (w : positive) (v1 v2 : @bit_int w),
   unsigned v1 = unsigned v2 -> v1 = v2.
 Proof.
-  intros v1 v2 H.
-  destruct v1 as [val1 range1].
-  destruct v2 as [val2 range2].
+  intros w v1 v2 H.
+  destruct v1, v2.
   apply mkint_eq; auto.
 Qed.
 
@@ -25,34 +25,4 @@ Proof.
   injection Heq as H_val_eq.
   apply H.
   assumption.
-Qed.
-
-Lemma uint8_concrete_if_else : forall (v1 v2 : uint8),
-  ((if eq v1 v2 then true else false) = true)->
-  v1 = v2.
-Proof.
-  intros v1 v2 H.
-  destruct (eq v1 v2) eqn:Ex.
-  -- unfold eq in Ex.
-     unfold Rocqlib.zeq in Ex.
-     destruct (Z.eq_dec (unsigned v1) (unsigned v2)) as [Heq|Hneq].
-     ---- apply uint8_eq_from_unsigned in Heq. rewrite Heq.
-          reflexivity.
-     ---- exfalso. congruence.
-  -- exfalso. congruence.
-Qed.
-
-Lemma uint8_concrete_if_else2 : forall (v1 v2 : uint8),
-  ((if eq v1 v2 then true else false) = false)->
-  v1 <> v2.
-Proof.
-  intros v1 v2 H.
-  destruct (eq v1 v2) eqn:Ex.
-  -- exfalso. congruence.
-  -- unfold eq in Ex.
-     unfold Rocqlib.zeq in Ex.
-     destruct (Z.eq_dec (unsigned v1) (unsigned v2)) as [Heq|Hneq].
-     --- exfalso. congruence.
-     --- apply uint8_neq_from_unsigned in Hneq.
-         assumption.            
 Qed.
